walk, cyclicity portion

main.v
@@ -6,11 +6,12 @@ Module Part1.
 (* Representation of Graph *)
 Notation Node := nat.
 Definition Edge := (prod Node Node).
-Definition EdgeList := (list Edge).
-(* Type edge. *)
+(* Adjacency List representation of Graph *)
 Definition Graph := list (prod Node (list Node)).
+(* Edge representation of Graph *)
+Definition EdgeGraph := list (prod Node Node).
 
-(* TODO := add the check to avoid duplicated edge addition *)
+(* Adding a edge to the graph *)
 Fixpoint add_edge (adj : Graph) (v1 v2: Node): Graph :=
     match adj with
     | nil => (cons (v1, (cons v2 nil)) nil) 
@@ -33,7 +34,9 @@ Proof.
 Qed.
 
 
-(* TODO --> check that we are not adding a node that's larger than n *)
+(* 
+    Functions to construct undirected and directed graphs 
+*)
 Fixpoint construct_undir_graph (n: nat) (edge_list : list Edge): Graph := 
     match edge_list with 
     | nil => (construct_empty_graph n)
@@ -46,6 +49,7 @@ Fixpoint construct_dir_graph (n: nat) (edge_list : list Edge): Graph :=
     | (cons (u,v) edge_list1) => add_edge (construct_dir_graph n edge_list1) u v
     end.
 
+(* Example checks for graph construction *)
 Example null_graph:=
     construct_undir_graph 0 nil.
 Example null_graph_is_null:
@@ -53,7 +57,6 @@ Example null_graph_is_null:
 Proof.
     auto.
 Qed.
-
 
 Example two_cycle:=
     construct_undir_graph 2 [(1,2)].
@@ -72,12 +75,7 @@ Proof.
 Qed.
 
 
-
-
-(* Todo  ---> Prove that construct_graph function is correct. *)
-
-
-
+(* Function to get all neighbors *)
 Fixpoint get_all_neighbors (g: Graph) (u : Node): (list Node):=
     match g with
     | nil => nil
@@ -90,7 +88,9 @@ Fixpoint get_all_neighbors (g: Graph) (u : Node): (list Node):=
                         then v::n1
                     else n1
     end.
-
+(* 
+    Function to get immediate children of a node
+*)
 Fixpoint get_children (g: Graph) (u : Node): (list Node):=
     match g with
     | nil => nil
@@ -101,7 +101,7 @@ Fixpoint get_children (g: Graph) (u : Node): (list Node):=
                 get_children g1 u
     end.
 
-
+(* Example checks for neighbors *)
 Example all_nghbrs_of_1_in_two_cycle:
     get_all_neighbors two_cycle 1 = [2].
 Proof.
@@ -120,7 +120,9 @@ Proof.
     simpl. auto.
 Qed.
 
-
+(*
+    Function to check if a given adjacency list representation of a graph is connected or not
+*)
 Fixpoint is_connected (g : Graph) : Prop:=
     match g with 
     | nil => True
@@ -131,8 +133,8 @@ Fixpoint is_connected (g : Graph) : Prop:=
                     end
     end.
     
-    
 
+(* Example checks *)
 Example null_graph_is_connected:
     is_connected null_graph.
 Proof.
@@ -154,6 +156,9 @@ Proof.
     simpl. auto.
 Qed.
 
+(* 
+    Following are the implemenation for edge represenatation of a graph
+ *)
 Definition node_in (g: Graph) (n : Node) : Prop :=
     exists edge_list, In (n, edge_list) g.
 
@@ -171,20 +176,19 @@ Qed.
 
 (* RETURNS True if u->v in the graph g *)
 Definition edge_in (g: Graph) (u : Node) (v : Node) : Prop :=
-    forall ngbhrs_list, In (u, ngbhrs_list) g  ->  In v ngbhrs_list.
+    node_in g u /\ (forall ngbhrs_list,  (In (u, ngbhrs_list) g  ->  In v ngbhrs_list)).
 
-(* g = [(1, [2,3,4]), (3, [4,5])] *)
-(* g = [(1, [2,3,4]), (3, [4,5]), (1, [5])]  -- this does not exist in our exmaplewas*) 
-(* edge_in g 1 2 = True *)
-(* edge_in g 2 1 = False *)
 
-    (* exists edge_list, (In (u, edge_list) g  /\  In v edge_list). *)
+Example two_in_one_line:
+    node_in one_line 2.
+Proof.
+    simpl. unfold node_in. unfold one_line. simpl. eauto.
+Qed.
 
 Example one_two_in_one_line:
     edge_in one_line 1 2.
 Proof.
-    (* simpl. unfold edge_in. unfold one_line. simpl. intros. split. destruct (1, edge_list). inversion H. easy. inversion H0. inversion H1. apply in_eq. easy.  *)
-    simpl. unfold edge_in. unfold one_line. simpl. intros. inversion H. easy. inversion H0. inversion H1. apply in_eq. easy. 
+    simpl. unfold edge_in. simpl. intros. split. apply one_in_one_line.  intros. inversion H. easy. inversion H0. inversion H1. apply in_eq. easy. 
 Qed.
 
 Example two_one_not_in_one_line:
@@ -193,16 +197,57 @@ Proof.
     intros .
     unfold edge_in in H.
     unfold one_line in H.
-    simpl in H.
-    specialize (H []).
+    simpl in H. destruct H. 
+    specialize (H0 []).
     firstorder.
 Qed.
 
 Example one_three_not_in_one_line:
     edge_in one_line 1 3 -> False.
 Proof.
-    unfold not. simpl. unfold edge_in. unfold one_line. simpl. intros. eauto. specialize (H [2]). firstorder. easy.
+    unfold not. simpl. unfold edge_in. unfold one_line. simpl. intros. destruct H. eauto. specialize (H0 [2]). firstorder. lia. easy.
 Qed.
+
+Fixpoint adj_graph_to_edge_list_helper (u: Node) (edge_list: list Node): EdgeGraph := 
+    match edge_list with 
+    | nil => nil
+    | (cons v edge_list_rest) => (u,v)::(adj_graph_to_edge_list_helper u edge_list_rest)
+    end.
+
+Fixpoint adj_graph_to_edge_list (graph: Graph): EdgeGraph := 
+    match graph with 
+    | nil => nil
+    | (cons (u,edge_list) rest_adj) => ((adj_graph_to_edge_list_helper u edge_list) ++ (adj_graph_to_edge_list rest_adj))
+    end.
+
+Compute adj_graph_to_edge_list [(1,[2;3;4]);(2,[3;4])].
+Lemma adj_reprsn_has_edge_list_reprsn: 
+    forall adj_graph, (exists edge_graph, (forall u v , edge_in adj_graph u v -> In (u, v) edge_graph)).
+Proof.
+intros.
+(* exists (adj_graph_to_edge_list adj_graph). *)
+intros.
+induction adj_graph.
+- exists (adj_graph_to_edge_list []). simpl. unfold edge_in. intros. destruct H. inversion H. firstorder.
+- exists (let (u, edge_list):=a in (adj_graph_to_edge_list_helper u edge_list) ++ (adj_graph_to_edge_list adj_graph)). intros. destruct a. eapply in_app_iff. inversion H; subst; clear H. inversion H0; subst; clear H0. inversion H. inversion H0; subst; clear H0.
+Admitted.
+
+Compute max 2 3.
+Fixpoint max_vertex (graph: EdgeGraph): Node :=
+    match graph with
+    | nil => 0
+    | (u,v)::rest_edge_list => max u (max v (max_vertex rest_edge_list)) 
+    end.
+
+Compute max_vertex [(1,2);(2,4);(4,5);(1,3)].
+
+Definition edge_list_to_adj_graph (graph: EdgeGraph): Graph := 
+    construct_dir_graph (max_vertex graph) graph.
+
+Lemma edge_reprsn_has_adj_graph_reprsn: 
+    forall edge_graph, (exists adj_graph, (forall u v , In (u, v) edge_graph -> edge_in adj_graph u v)).
+Proof.
+Admitted.
 
 
 Inductive is_reachable_ind : Graph -> Node -> Node -> Prop :=
@@ -228,65 +273,11 @@ Proof.
     intros.
 Admitted.
 
-
 Example one_cycle:=
     construct_dir_graph 2 [(1,2);(2,1)].
 
 Example one_loop:=
     construct_dir_graph 2 [(1,1)].
-
-Example one_one_reachable_in_one_cycle:
-    is_reachable_ind one_cycle 1 1.
-Proof.
-    eapply is_reachable_ind_once. unfold one_cycle. simpl. unfold edge_in. intros. inversion H. firstorder. easy. easy. firstorder.  easy. inversion H. firstorder.
-    eapply is_reachable_ind_base. unfold one_cycle. simpl. unfold edge_in. intros. inversion H. firstorder. inversion H. firstorder. easy. firstorder. easy.  easy.
-Qed.
-
-Example two_two_reachable_in_one_cycle:
-    is_reachable_ind one_cycle 2 2.
-Proof.
-    eapply is_reachable_ind_once. unfold one_cycle. simpl. unfold edge_in. intros. inversion H. firstorder. inversion H. firstorder. easy. firstorder. easy. firstorder.  easy.
-    eapply is_reachable_ind_base. unfold one_cycle. simpl. unfold edge_in. intros. inversion H. firstorder. inversion H. firstorder. easy. firstorder. easy. inversion H.  firstorder.
-Qed.
-
-
-
-
-Definition is_cyclic_ind (g: Graph) : Prop :=
-    exists v, node_in g v /\ is_reachable_ind g v v.
-    (* The following does not work because false is difficult to prove *)
-    (* exists v, node_in g v -> is_reachable_ind g v v. *)
-
-Example one_line_is_not_cyclic:
-    ~ (is_cyclic_ind one_line).
-Proof.
-    unfold is_cyclic_ind. unfold not. firstorder. inversion H; subst; clear H. apply two_two_not_reachable_ind_in_one_line in H0. firstorder. inversion H; subst; clear H. apply one_one_not_reachable_ind_in_one_line in H0. firstorder.
-Qed.
-
-
-Example one_cycle_is_cyclic:
-    is_cyclic_ind one_cycle.
-Proof.
-    exists 1. split. 
-    unfold node_in. unfold one_cycle. simpl. exists [2]. firstorder.
-    apply one_one_reachable_in_one_cycle.
-Qed.
-
-Definition is_dag (g:Graph) : Prop :=
-    is_cyclic_ind g -> False.
-
-
-
-Definition no_parent (g:Graph) (v:Node) : Prop :=
-    forall v1, node_in g v1 -> ~ edge_in g v1 v.
-
-Example one_has_noparent_in_one_line:
-    no_parent one_line 1.
-Proof.
-    unfold no_parent. firstorder. inversion H; subst; clear H. unfold not. intros. unfold one_line in H. unfold edge_in in H. simpl in H. specialize (H []). firstorder.
-    inversion H; subst; clear H.
-    unfold not. intros. unfold one_line in H. unfold edge_in in H. simpl in H. specialize (H [2]). firstorder. easy.
-Qed.
 
 
 (* ----------------------------------------------------------------------- *)
@@ -805,130 +796,6 @@ Example diameter_longest_path :
 Proof. reflexivity. Qed.
 
 
-(* Additional Properties and some extensions for Graph *)
-
-(* Walk in a graph *)
-Inductive is_walk: Graph -> list Node -> Prop :=
-| walkOne : forall  g v, node_in g v -> is_walk g [v]
-| walkOneStep : forall g u v l, edge_in g u v -> is_walk g (v::l) -> is_walk g (u :: v :: l).
-
-Inductive has_no_duplicates: list Node -> Prop :=
-| emptyNoDuplicates : has_no_duplicates []
-| nonEmptyNoDuplicates: forall v l, not (In v l) -> has_no_duplicates (v::l).
-
-Fixpoint tail_elem (l : list Node) :=
-  match l with
-  | [] => error
-  | [x] => Some x
-  | _ :: xs => tail_elem xs
-  end.
-
-Goal tail_elem [2;3;4] = Some 4.
-Proof.
-firstorder.
-Qed.
-
-Goal head [2;3;4] = Some 2.
-Proof.
-firstorder.
-Qed.
-
-(* Inductive head_tail_same : list Node -> Prop :=
-| emptyHeadTailSame : head_tail_same []
-| nonEmptyHeadTailSame: forall a l, head_tail_same (a::(l++[a])).
-
-Compute (1::([2;3;4]++[5])).
-
-Goal head_tail_same [1;2;1].
-(* Goal head_tail_same (1::([2]++[1])). *)
-Proof.
-eapply nonEmptyHeadTailSame. *)
-
-
-Definition head_tail_same (l : list Node) :=
-    length l >= 2 /\ ((head l) = (tail_elem l)).
-
-Goal head_tail_same [2;3;2].
-Proof.
-unfold head_tail_same. split. unfold length. lia. firstorder.
-Qed.
-
-    
-Definition is_path (g:Graph) (l: list Node) : Prop :=
-    is_walk g l /\ has_no_duplicates l.
-
-
-Definition is_cycle (g:Graph) (l: list Node) : Prop :=
-        is_walk g l /\ head_tail_same l.
-
-Lemma head_tail_same_implies_duplicates:
-    forall l, head_tail_same l -> not ( has_no_duplicates l).
-Proof.
-induction l.
-- unfold head_tail_same. intros. destruct H. simpl in H. firstorder. easy.
--intros. destruct H. 
-Admitted.
-
-Lemma path_is_not_cycle: 
-    forall g l, is_path g l -> not (is_cycle g l).
-Proof.
-    (* induction l.
-    - unfold not. intros. inversion H; subst; clear H. inversion H0; subst; clear H0. unfold head_tail_same in H3. inversion H3. simpl in H0. lia.
-    - intros. unfold not.  intros. inversion H . eapply walkOneStep in H1. inversion H2. simpl in H. *)
-    intros. unfold not, is_path, is_cycle. destruct H. intros. destruct H1. eapply head_tail_same_implies_duplicates in H0. easy. easy.
-Qed.
-
-Lemma maximal_path_exists_in_dag:
-    forall g l , is_dag g -> (exists max_path, (is_path g max_path) /\ ((is_path g l) -> (length l <= length max_path ))).
-Proof.
-Admitted.
-
-
-    
-        
-(* The following theorem requires knowledge that a path of maximum length occurs in a dag *)
-Theorem dag_has_atleast_one_root: 
-    forall g, is_dag g -> (exists v, node_in g v /\ no_parent g v).
-Proof.
-    intros. firstorder. 
-Admitted.
-
-(* Forest *)
-
-Definition is_forest (g:Graph) : Prop :=
-    is_dag g /\ (forall p1 p2 v, node_in g v -> (edge_in g p1 v -> edge_in g p2 v  -> p1 = p2)).
-    
-Example is_line_is_forest:
-    is_forest one_line.
-Proof.
-    split.
-    unfold is_dag. apply one_line_is_not_cyclic.
-    unfold one_line. simpl. unfold edge_in. intros. firstorder. inversion H; subst; clear H. unfold edge_in in H1. destruct p1.
-Admitted.
-
-Definition is_connected_ind (g: Graph) : Prop :=
- forall u v, (not (u = v) /\ node_in g u /\ node_in g v) -> (is_reachable_ind g u v  \/ is_reachable_ind g v u).
-
-
-(* Is Graph a Tree *)
-
-Definition is_tree (g: Graph):
-    is_forest g /\ is_connected_ind g.
-
-
-
-Definition is_leaf (g:Graph) (v: Node) :Prop :=
-    (node_in g v) /\ (In (v, []) g).
-
-Proof.
-Admitted.
-
-
-Theorem tree_has_1_less_internal_nodes_than_leaves:
-    True.
-Proof.
-Admitted.
-
 (*=============== DFS ==================*)
 
 (*  Small Step Semantics Definition of DFS *)
@@ -1259,3 +1126,199 @@ Proof.
       auto.
 Qed.
 
+
+
+(* 
+    Additional Properties and some extensions for Graph 
+*)
+
+(* Walk in a graph *)   
+Inductive is_walk: Graph -> list Node -> Prop :=
+| walkOne : forall  g v, node_in g v -> is_walk g [v]
+| walkOneStep : forall g u v l, edge_in g u v -> is_walk g (v::l) -> is_walk g (u :: v :: l).
+
+Inductive has_no_duplicates: list Node -> Prop :=
+| emptyNoDuplicates : has_no_duplicates []
+| nonEmptyNoDuplicates: forall v l, not (In v l) -> has_no_duplicates (v::l).
+
+Fixpoint tail_elem (l : list Node) :=
+  match l with
+  | [] => error
+  | [x] => Some x
+  | _ :: xs => tail_elem xs
+  end.
+
+
+Goal tail_elem [2;3;4] = Some 4.
+Proof.
+firstorder.
+Qed.
+
+Goal head [2;3;4] = Some 2.
+Proof.
+firstorder.
+Qed.
+
+
+Fixpoint has_duplicates (l:list Node): Prop :=
+    match l with 
+    | nil => False
+    | a::l1 => In a l1 \/ (has_duplicates l1)
+    end.
+
+    Goal not (has_duplicates [1;2;3]).
+    Proof.
+    unfold not. firstorder. easy. easy. easy.
+    Qed.
+    
+    Goal has_duplicates [1;2;1;3].
+    Proof.
+    firstorder. 
+    Qed.
+    
+        
+Definition head_tail_same (l : list Node) :=
+    (length l >=2) /\ (head l) = (tail_elem l).
+
+    Goal head_tail_same [2;3;2].
+    Proof.
+    firstorder. simpl. lia.
+    Qed.
+    
+    Goal not (head_tail_same [2]).
+    Proof.
+    unfold head_tail_same. firstorder. simpl. lia.
+    Qed.
+
+    Goal not( head_tail_same []).
+    Proof.
+    unfold not. unfold head_tail_same. firstorder. simpl in H. lia.
+    Qed.
+
+            
+Definition is_path (g:Graph) (l: list Node) : Prop :=
+    is_walk g l /\ (not (has_duplicates l)).
+
+
+(* 
+    Definition of cyclicity in graph
+*)
+Definition is_cycle (g:Graph) (l: list Node) : Prop :=
+        length l>=2 /\ is_walk g l /\ head_tail_same l.
+
+Lemma head_tail_same_implies_duplicates:
+    forall l, head_tail_same l -> has_duplicates l.
+Proof.
+intros. inversion H; subst;clear H. 
+(* assert (exists a l1, a::l1=l). inversion H0. inversion H2. 
+induction l.
+- unfold head_tail_same. intros. simpl in H. firstorder. easy.
+- intros. firstorder. simpl in H. inversion H; subst; clear H. destruct l. simpl in H. lia. simpl in H1. assert (In a (n::l)). simpl in H0.  *)
+Admitted.
+
+
+Lemma path_is_not_cycle: 
+    forall g l, is_path g l -> not (is_cycle g l).
+Proof.
+    intros. unfold not, is_path, is_cycle. destruct H. intros. destruct H1. destruct H2. apply head_tail_same_implies_duplicates in H3. contradiction.
+Qed.
+Lemma cycle_is_not_path: 
+    forall g l, is_cycle g l -> not (is_path g l).
+Proof.
+    intros. unfold not, is_path, is_cycle. destruct H. intros. destruct H1. destruct H0. apply head_tail_same_implies_duplicates in H3. contradiction.
+Qed.
+
+
+Definition is_reachable_walk (g:Graph) (u:Node) (v:Node): Prop :=
+ exists walk, (length walk >=2) /\ is_walk g walk /\ ((head walk) = Some u) /\ ((tail_elem walk) = Some v).
+
+Definition is_cyclic (g: Graph) : Prop :=
+    exists l, is_cycle g l.
+    (* The following does not work because false is difficult to prove *)
+    (* exists v, node_in g v -> is_reachable_ind g v v. *)
+
+Definition is_dag (g:Graph) : Prop :=
+    is_cyclic g -> False.
+
+Lemma in_dag_no_node_is_reachable_to_itself:
+    forall g v, is_dag g -> node_in g v -> (not (is_reachable_walk g v v)).
+Proof.
+intros. unfold not. firstorder. (* Assuming a walk exists that starts and ends at the same node *)
+ assert (is_cycle g x). firstorder. rewrite H4. firstorder. (* Proving that the walk should be a cycle*)  
+ specialize (H x). simpl in H. firstorder. (* Proving that presence of a cylce contradicts that the graph is a DAG *)
+Qed. 
+
+
+Example one_cycle_is_cyclic:
+    is_cyclic one_cycle.
+Proof.
+    unfold is_cyclic. exists [1;2;1]. firstorder. simpl. lia. eapply walkOneStep. firstorder. unfold one_cycle. simpl. unfold node_in. exists [2]. firstorder.
+    inversion H. inversion H. firstorder.
+    eapply walkOneStep. firstorder. unfold one_cycle. simpl. unfold node_in. exists [1]. firstorder.
+    inversion H. inversion H. firstorder.
+    inversion H. eapply walkOne. unfold one_cycle. simpl. unfold node_in. exists [2]. firstorder. simpl. lia.
+Qed.
+
+
+Definition no_parent (g:Graph) (v:Node) : Prop :=
+    forall v1, node_in g v1 -> ~ edge_in g v1 v.
+
+Definition is_root (g:Graph) (v:Node) : Prop :=
+    no_parent g v.
+
+Example one_has_noparent_in_one_line:
+    no_parent one_line 1.
+Proof.
+    unfold no_parent. firstorder. inversion H; subst; clear H. unfold not. intros. unfold one_line in H. unfold edge_in in H. simpl in H. destruct H. specialize (H0 []). firstorder.
+    inversion H; subst; clear H.
+    unfold not. intros. unfold one_line in H. unfold edge_in in H. destruct H. simpl in H. specialize (H0 [2]). firstorder. easy. lia.
+Qed.
+
+
+Lemma maximal_path_exists_in_dag:
+    forall g , is_dag g -> (exists max_path, forall l, (is_path g max_path) /\ ((is_path g l) -> (length l <= length max_path ))).
+Proof.
+ intros.
+Admitted.
+
+
+
+(* The following theorem requires knowledge that a path of maximum length occurs in a dag *)
+Theorem dag_has_atleast_one_root: 
+    forall g, is_dag g -> (exists v, node_in g v /\ no_parent g v).
+Proof.
+    intros.  apply  maximal_path_exists_in_dag in H. destruct H. 
+Admitted.
+
+Definition is_leaf (g:Graph) (v: Node) :Prop :=
+    (node_in g v) /\ (In (v, []) g).
+
+(* The following theorem requires knowledge that a path of maximum length occurs in a dag *)
+(* Theorem dag_has_atleast_one_leaf: 
+    forall g, is_dag g -> (exists v, is_leaf g v).
+Proof.
+Admitted. *)
+
+(* Forest *)
+
+Definition is_forest (g:Graph) : Prop :=
+    is_dag g /\ (forall p1 p2 v, node_in g v -> (edge_in g p1 v -> edge_in g p2 v  -> p1 = p2)).
+    
+Example is_line_is_forest:
+    is_forest one_line.
+Proof.
+    split.
+    unfold is_dag. 
+    (* apply one_line_is_not_cyclic. *)
+    unfold one_line. simpl. unfold edge_in. intros. firstorder. inversion H; subst; clear H. unfold edge_in in H1. 
+    (* destruct p1. *)
+Admitted.
+
+Definition is_connected_ind (g: Graph) : Prop :=
+ forall u v, not (u = v) -> (is_reachable_walk g u v).
+
+
+(* Attempt to expand graph as trees: Is Graph a Tree *)
+
+Definition is_tree (g: Graph):
+    is_forest g /\ is_connected_ind g.
